WebAssembly/Wasm_Monad_Printing.thy
@@ -31,27 +31,7 @@ proof -
     apply (simp add: drop_bit_take_bit)
     by (metis add_diff_cancel_left' drop_bit_mask_eq min_minus min_pm1 take_bit_of_mask)
 qed
-
-fun run_fuzz :: "fuel \<Rightarrow> depth \<Rightarrow> s_m \<Rightarrow> m \<Rightarrow> v_ext list \<Rightarrow> (v list) option \<Rightarrow> (s_m \<times> res) Heap" where
-  "run_fuzz n d s m v_imps opt_vs = do {
-   i_res \<leftarrow> interp_instantiate_init_m s m v_imps;
-   case i_res of
-     (s', RI_res_m inst v_exps init_es) \<Rightarrow>
-     (case (List.find (\<lambda>exp. case (E_desc exp) of Ext_func i \<Rightarrow> True | _ \<Rightarrow> False) v_exps) of
-        Some exp \<Rightarrow> (case (E_desc exp) of Ext_func i \<Rightarrow> do {
-                       cl \<leftarrow> Array.nth (s_m.funcs s') i;
-                       case (cl_m_type cl) of
-                         (t1 _> t2) \<Rightarrow>
-                           let params = case opt_vs of Some vs \<Rightarrow> (rev vs) | None \<Rightarrow> (map bitzero t1) in
-                           run_invoke_v_m n d (s', params, i) })
-      | None \<Rightarrow> return (s', RCrash (Error_invariant (STR ''no import to invoke''))))
-  | (s', RI_crash_m res) \<Rightarrow> return (s', RCrash res)
-  | (s', RI_trap_m msg) \<Rightarrow> return (s', RTrap msg) }"
-
-fun run_fuzz_entry :: "fuel \<Rightarrow> m \<Rightarrow> (v list) option \<Rightarrow> (s_m \<times> res) Heap" where
-  "run_fuzz_entry n m vs_opt = do {
-     s_m \<leftarrow> make_empty_store_m;
-     run_fuzz n 300 s_m m [] vs_opt }"
+   
 
 export_code open nat_of_byte byte_of_nat
                  ocaml_int32_to_isabelle_int32
